$$Mat_{e}(x) = \begin{pmatrix}
e_{i}^{*}(x_{j})
\end{pmatrix}_{i, j}$$
$$Mat_{e, f}(u) = Mat_{f}(u(e))$$

___
$$\begin{cases}
A = Mat_{e, f}(u) \\
X = Mat_{e}(x) \\
Y = Mat_{f}(u(x))
\end{cases}$$
$$Y = AX$$
___
$$Mat_{e, g}(v \circ u) = Mat_{f, g}(v)Mat_{e, f}(u)$$
$$Mat_{f, e}(u^{-1}) = (Mat_{e, f}(u))^{-1}$$
___
$$\begin{cases}
P = P_{e}^{e'} \\
X = Mat_{e}(x) \\
X' = Mat_{e'}(x)
\end{cases}$$
$$X = PX'$$
___
$$\begin{cases}
P = P_{e}^{e'} \\
Q = P_{f}^{f'} \\
A = Mat_{e, f}(u) \\
A' = Mat_{e', f'}(u)
\end{cases}$$
$$A'=Q^{-1}AP$$
___
